Fix new KS interface in HS

src/tls/Epochs.fst
@@ -118,12 +118,23 @@ val set_reader: #r:rgn -> #n:TLSInfo.random ->
        (ensures (fun h0 x h1 -> True))
 let set_reader #r #n (Epochs es r w) i' = r := i'
 
+val incr_reader: #r:rgn -> #n:TLSInfo.random ->
+               es:epochs r n -> ST unit
+       (requires (fun h -> True))
+       (ensures (fun h0 x h1 -> True))
+let incr_reader #r #n (Epochs es r w) = r := !r + 1
 
 val set_writer: #r:rgn -> #n:TLSInfo.random -> 
     	       es:epochs r n -> i:nat -> ST unit
        (requires (fun h -> True))
        (ensures (fun h0 x h1 -> True))
 let set_writer #r #n (Epochs es r w) i' = w := i'
+
+val incr_writer: #r:rgn -> #n:TLSInfo.random ->
+               es:epochs r n -> ST unit
+       (requires (fun h -> True))
+       (ensures (fun h0 x h1 -> True))
+let incr_writer #r #n (Epochs es r w) = w := !w + 1
 
 let get_epochs (Epochs es r w) = es 
 
